

~~1~~ - ①

SOME SOLVE PROBLEMS

① Consider the Complex Series

$$\sum_{k=1}^{\infty} \frac{\sinh kz}{k^2},$$

show that it is absolutely convergent when z is real but it becomes divergent when z is non-real.

Solution

(a) When z is real, we have

$$\left| \frac{\sinh kz}{k^2} \right| \leq \frac{1}{k^2} \quad \forall k > 0, k \in \mathbb{Z}.$$

Since $\sum_{k=1}^{\infty} \frac{1}{k^2}$ is known to be convergent,

then $\sum_{k=1}^{\infty} \frac{\sinh kz}{k^2}$ is absolutely convergent $\forall z$

by virtue of the Comparison test.

(b) When z is non-real, we let $z = x + iy$, $y \neq 0$

$$\text{Hence, } \frac{\sinh kz}{k^2} = \frac{e^{-ky} e^{ikx} - e^{ky} e^{-ikx}}{2k^2 i},$$

we deduce that

$$\left| \frac{\sinh kz}{k^2} \right| \geq \frac{e^{k|y|} - e^{-k|y|}}{2k^2} \rightarrow \infty \text{ as } k \rightarrow \infty$$

Since $\left| \frac{\sinh kz}{k^2} \right|$ is unbounded as $k \rightarrow \infty$, the series is divergent.

② Find the Circle of Convergence for each of the following power series:

(a) $\sum_{k=1}^{\infty} \frac{1}{k} (z-i)^k$

Solution

By the ratio test, we have

$$R = \lim_{k \rightarrow \infty} \frac{1/k}{1/(k+1)} = 1$$

\therefore the circle of conv. is $|z-i|=1$

(b) $\sum_{k=1}^{\infty} k^{\ln k} (z-2)^k$

using the root test, we have

$$\frac{1}{R} = \lim_{k \rightarrow \infty} \sqrt[k]{|a_k|} = \lim_{k \rightarrow \infty} \sqrt[k]{k^{\ln k}}$$

To evaluate the limit, we consider the logarithm,

$$\ln \left(\lim_{k \rightarrow \infty} \sqrt[k]{k^{\ln k}} \right) = \lim_{k \rightarrow \infty} \ln \left(\sqrt[k]{k^{\ln k}} \right) = \lim_{k \rightarrow \infty} \frac{(\ln k)^2}{k} = 0$$

$$\text{So, } \frac{1}{R} = \lim_{k \rightarrow \infty} \sqrt[k]{k^{\ln k}} = e^0 = 1$$

\therefore The Circle of conv. is $|z-2|=1$.

~~2~~ (2)

$$(c) \sum_{k=1}^{\infty} \left(\frac{z}{k}\right)^k$$

Solution

By the ratio Test, we have

$$R = \lim_{k \rightarrow \infty} \frac{\left(\frac{1}{k}\right)^k}{\left(\frac{1}{k+1}\right)^{k+1}} = \lim_{k \rightarrow \infty} (k+1) \left(1 + \frac{1}{k}\right)^k = \infty$$

So the circle of conv. is the whole complex plane.

$$(d) \sum_{k=1}^{\infty} \left(1 + \frac{1}{k}\right)^{k^2} \cdot z^k$$

Solution

By the root test, we have

$$\frac{1}{R} = \lim_{k \rightarrow \infty} \sqrt[k]{\left(1 + \frac{1}{k}\right)^{k^2}} = \lim_{k \rightarrow \infty} \left(1 + \frac{1}{k}\right)^k = e$$

\therefore the circle of conv. is $|z| = \frac{1}{e}$.

③ Find the Laurent expansion of

$$f(z) = \sin\left(z - \frac{1}{z}\right)$$

The function has singularity at $z=0$, so that the annulus of conv. is $|z| > 0$. The Laurent coefficient C_n is given by

$$C_n = \frac{1}{2\pi i} \oint_C \frac{\sin\left(z - \frac{1}{z}\right)}{z^{n+1}} dz, \quad n = 0, \pm 1, \pm 2, \dots$$

where C is chosen to be the unit circle $|z|=1$
 Take $z = e^{i\theta}$ so that $dz = ie^{i\theta} d\theta$, then

$$C_n = \frac{1}{2\pi i} \int_{-\pi}^{\pi} \frac{\sin(2i \sin \theta)}{e^{i(n+1)\theta}} d\theta$$

$$= \frac{1}{2\pi} \int_{-\pi}^{\pi} i \sinh(2 \sin \theta) (\cos n\theta - i \sin n\theta) d\theta.$$

Note that $\sinh(2 \sin \theta)$ is an odd function in θ , hence,

$$\int_{-\pi}^{\pi} \sinh(2 \sin \theta) \cos n\theta d\theta = 0.$$

Finally,

$$C_n = \frac{1}{2\pi} \int_{-\pi}^{\pi} \sinh(2 \sin \theta) \sin n\theta d\theta, \quad n = 1, \pm 1, \pm 2, \dots$$

(4) Find the Laurent Expansion of

$$f(z) = \frac{1}{z-k}$$

That is valid in the domain $|z| > k$, where k is real and $|k| < 1$. Using the Laurent expansion, deduce that

$$\sum_{k=1}^{\infty} k^n \cos n\theta = \frac{k \cos \theta - k^2}{1 - 2k \cos \theta + k^2},$$

$$\sum_{k=1}^{\infty} k^n \sin n\theta = \frac{k \sin \theta}{1 - 2k \cos \theta + k^2}$$

~~Ques~~ (3)

Solution

For $|z| > k$, where $|k| < 1$, we have

$$\frac{1}{z-k} = \frac{1}{z(1-\frac{k}{z})}$$

$$= \frac{1}{z} \left(1 + \frac{k}{z} + \frac{k^2}{z^2} + \dots \right) \text{ for } \left| \frac{k}{z} \right| < 1$$

Take the point $z = e^{i\theta}$, which lies inside the region of conv. of the above Laurent Series, substituting into infinite Series

$$\frac{1}{e^{i\theta} - k} = \frac{1}{e^{i\theta}} \left(1 + k e^{-i\theta} + k^2 e^{-2i\theta} + \dots + k^n e^{-in\theta} + \dots \right)$$

Rearranging the terms

$$\frac{e^{i\theta}(e^{-i\theta} - k)}{(e^{i\theta} - k)(e^{-i\theta} - k)} = \frac{1 - k(\cos\theta + i\sin\theta) - (1 - 2k\cos\theta + k^2)}{1 - 2k\cos\theta + k^2}$$

$$= \frac{k\cos\theta - k^2 - ik\sin\theta}{1 - 2k\cos\theta + k^2}$$

$$= \sum_{n=1}^{\infty} k^n \cos n\theta - i \sum_{n=1}^{\infty} k^n \sin n\theta$$

Equating the real and imaginary parts, we obtain the desired results.

⑤ By evaluating the contour integral

$$\oint_{|z|=1} \left(z + \frac{1}{z}\right)^{2n} \frac{dz}{z},$$

show that

$$\int_0^{2\pi} \cos^{2n}(\theta) d\theta = 2\pi \frac{1 \cdot 3 \cdot 5 \dots (2n-1)}{2 \cdot 4 \cdot 6 \dots 2n}$$

Solution

on $|z|=1$, $z = e^{i\theta}$; $\left(z + \frac{1}{z}\right)^{2n} = 2^{2n} \cos^{2n} \theta$; $\frac{dz}{z} = i d\theta$

$$I = \oint_{|z|=1} \left(z + \frac{1}{z}\right)^{2n} \frac{dz}{z} = 2^{2n} i \int_0^{2\pi} \cos^{2n}(\theta) d\theta$$

on the other hand, the integrand can be expanded as

$$\frac{1}{z} \left(z^{2n} + 2nC_1 z^{2n-2} + \dots + 2nC_n + \dots + 2nC_{2n} \frac{1}{z^{2n}} \right), \quad 0 < |z| < \infty$$

Since the integrand is analytic everywhere except at $z=0$, the above expansion is the Laurent Series of the integrand valid in the annulus: $|z| > 0$.

$$\oint_{|z|=1} \left(z + \frac{1}{z}\right)^{2n} \frac{dz}{z} = 2\pi i \left(\text{coefficient of } \frac{1}{z} \text{ in the Laurent Series} \right)$$

$$= 2\pi i 2n C_n.$$

Hence,

~~4~~ - (4)

$$\int_0^{2\pi} \cos^{2n}(\theta) d\theta = 2\pi \frac{2n C_n}{2^{2n}}$$

$$= 2\pi \frac{(2n)!}{(n!)^2 2^{2n}}$$

$$= 2\pi \frac{1 \cdot 3 \cdot 5 \cdot \dots \cdot (2n-1)}{2 \cdot 4 \cdot 6 \cdot \dots \cdot (2n)}$$

⑥ For each of the following complex functions, do the following:

- find all its singularities in \mathbb{C}
- write the principal part of the function at each singularity;
- for each singularity, determine whether it is a pole, a removable singularity, or an essential singularity
- compute the residue of the function at each singularity.

6.1) $f(z) = \frac{1}{(\cos z)^2}$

Solution

$f(z)$ is singular at $\cos z = 0$, i.e., $z = n\pi + \frac{\pi}{2}$

Let $w = z - n\pi - \frac{\pi}{2}$

Then

$$\frac{1}{(\cos z)^2} = \frac{1}{(\cos(w + n\pi + \frac{\pi}{2}))^2} = \frac{1}{(\sin w)^2}$$

Since $\sin w$ has a zero of multiplicity one at $w = 0$, $f(z)$ has a pole of order 2 at $z = n\pi + \frac{\pi}{2}$. So

$$\frac{1}{(\sin \omega)^2} = \frac{a_{-2}}{\omega^2} + \frac{a_{-1}}{\omega} + \sum_{n \geq 0} a_n \omega^n.$$

Since

$$(\sin \omega)^2 = \left(\sum_{n=0}^{\infty} \frac{(-1)^n \omega^{2n+1}}{(2n+1)!} \right)^2 = \omega^2 + \sum_{n=4}^{\infty} b_n \omega^n$$

we have

$$1 = \left(\frac{a_{-2}}{\omega^2} + \frac{a_{-1}}{\omega} + \sum_{n \geq 0} a_n \omega^n \right) \left(\omega^2 + \sum_{n=4}^{\infty} b_n \omega^n \right).$$

Comparing the coefficients of 1 and ω on both sides, we obtain

$$\frac{a_{-2}}{-2} = 1$$

$$\frac{a_{-1}}{-1} = 0$$

so the principal part of $f(z)$ at $z = n\pi + \frac{\pi}{2}$ is

$$\frac{1}{(z - n\pi - \frac{\pi}{2})^2}$$

with residue 0.

~~Ques~~ - (5)

Given $f(z) = \frac{\cos z}{z^2 - z^3}$

a) Find the principal part of $f(z)$

b) Find the Residue of $f(z)$

Solution

The function has singularities at $\{z^2 - z^3 = 0\}$
 $\Rightarrow \{z^2(1-z) = 0\} \Rightarrow z=0$ (pole of order 2)
 $z=1$ (single pole)

Suppose that the Laurent series of $f(z)$ at $z=0$ is given by

$$\frac{\cos z}{z^2 - z^3} = \frac{a_{-2}}{z^2} + \frac{a_{-1}}{z} + \sum_{n \geq 0} a_n z^n$$

$$\begin{aligned} \cos z &= \sum_{n=0}^{\infty} \frac{(-1)^n z^{2n}}{(2n)!} \\ &= \sum_{n=0}^{\infty} \frac{(-1)^n z^{2n}}{(2n)!} \\ &= 1 - \frac{z^2}{2!} + \frac{z^4}{4!} - \dots \end{aligned}$$

Hence,

$$(z^2 - z^3) \left(\frac{a_{-2}}{z^2} + \frac{a_{-1}}{z} + \sum_{n \geq 0} a_n z^n \right) = \cos z = 1 + \sum_{n=1}^{\infty} \frac{(-1)^n z^{2n}}{(2n)!}$$

Comparing the coefficient of 1 and z both sides, we obtain that:

$$a_{-2} = 1 \text{ and } a_{-1} - a_{-2} = 0. \text{ Hence } a_{-1} = a_{-2}$$

\therefore the principal part of $f(z)$ at $z=0$ is

$$\frac{1}{z^2} + \frac{1}{z}$$

$$(6) \operatorname{Res} f(z) = 1$$

$$\begin{aligned} \operatorname{Res} f(z) &= \lim_{z \rightarrow 0} \frac{1}{1!} \frac{d}{dz} \left\{ z^2 \frac{\cos z}{z^2 - z^3} \right\} \\ &= \lim_{z \rightarrow 0} \frac{d}{dz} \left\{ \frac{\cos z}{1-z} \right\} \\ &= \lim_{z \rightarrow 0} \frac{-\sin z(1-z) + \cos z(1-z)}{(1-z)^2} = \textcircled{1} \end{aligned}$$

(*) $z=1$ (Single pole)

$$\begin{aligned} a_{-1} = \operatorname{Res} f(z) &= \lim_{z \rightarrow 1} (z-1) \frac{\cos z}{z^2(1-z)} = - \lim_{z \rightarrow 1} \frac{\cos z}{z^2} = -\cos 1 \\ &= -\cos(1) \end{aligned}$$

$$\frac{\cos z}{z^2 - z^3} = \frac{a_{-1}}{(z-1)} + \sum_{n \geq 0} a_n z^n$$

Hence, the principal part of $f(z)$ at $z=1$ is

$$= \frac{\cos(1)}{z-1}.$$

~~XXXXXXXXXXXXXXXXXXXX~~